gen.v
@@ -34,6 +34,12 @@ Proof. intros. subst. reflexivity. Qed.
 Lemma arg_cong: forall T U f x y, x = y -> (f (x : U) : T) = f y.
 Proof. intros. subst. reflexivity. Qed.
 
+Lemma arg1_cong_imp: forall U V f x y z, x = y -> f (x : U) (z : V) -> f y z.
+Proof. intros. subst. assumption. Qed.
+
+Lemma arg_cong_imp: forall U f x y, x = y -> f (x : U) -> f y.
+Proof. intros. subst. assumption. Qed.
+
 Lemma iffD1: forall x y, (x = y) -> x -> y.
 Proof. intros.  subst.  assumption. Qed.
 
@@ -186,3 +192,4 @@ Proof. intros. unfold iff. rewrite Forall_forall.
 Lemma Forall_map_single: forall (A B : Type) P (f : A -> B) x, 
   Forall P (map f [x]) <-> P (f x).
 Proof.  simpl. intros. apply Forall_single. Qed.
+
